Anon1Assignment.lean
@@ -1,1 +1,5 @@
 import Anon1Assignment.Grader
+import Anon1Assignment.Student
+
+#eval Anon1.Student.solve [1,5,2]
+#eval Anon1.Student.solve [1,5,233,7]
